Common.v
@@ -4,3 +4,14 @@ Class Env {K V: Type}: Type :=
     putenv: env_t -> K -> V -> env_t }.
 Arguments Env : clear implicits.
 Arguments env_t {_ _}.
+
+Inductive Posed {P: Prop}: P -> Prop :=
+| AlreadyPosed : forall p: P, Posed p.
+
+Tactic Notation "pose_once" uconstr(thm) :=
+  (progress match goal with
+            | [ H: Posed ?thm' |- _ ] =>
+              unify thm thm'
+            | _ => pose proof thm;
+                  pose proof (AlreadyPosed thm)
+            end).
